src/Math/Measures.dfy
@@ -1,0 +1,175 @@
+/*******************************************************************************
+ *  Copyright by the contributors to the Dafny Project
+ *  SPDX-License-Identifier: MIT
+ *******************************************************************************/
+
+module Measures {
+  /************
+   Definitions
+  ************/
+
+  type Probability = x: real | 0.0 <= x <= 1.0
+
+  ghost predicate IsSigmaAlgebra<T(!new)>(eventSpace: iset<iset<T>>, sampleSpace: iset<T>) {
+    && (forall e | e in eventSpace :: e <= sampleSpace)
+    && (iset{}) in eventSpace
+    && (forall e | e in eventSpace :: (sampleSpace - e) in eventSpace)
+    && (forall f: nat -> iset<T> | (forall n :: f(n) in eventSpace) :: (CountableUnion(f) in eventSpace))
+  }
+
+  ghost function CountableUnion<T(!new)>(f: nat -> iset<T>, i: nat := 0): iset<T> {
+    iset n: nat | n >= i, x <- f(n) :: x
+  }
+
+  function CountableSum(f: nat -> real, i: nat := 0): real {
+    assume {:axiom} false; // assume termination
+    f(i) + CountableSum(f, i+1)
+  }
+
+  ghost const boolSampleSpace: iset<bool> := iset _: bool
+
+  ghost const boolEventSpace: iset<iset<bool>> := iset _: iset<bool>
+
+  ghost const natSampleSpace: iset<nat> := iset _: nat
+
+  // The sigma algebra on the natural numbers is just the power set
+  ghost const natEventSpace: iset<iset<nat>> := iset _: iset<nat>
+
+  // Definition 5
+  ghost predicate IsPositive<T(!new)>(eventSpace: iset<iset<T>>, Prob: iset<T> -> real) {
+    && Prob(iset{}) == 0.0
+    && forall e | e in eventSpace :: 0.0 <= Prob(e)
+  }
+
+  // Definition 5
+  ghost predicate IsAdditive<T(!new)>(eventSpace: iset<iset<T>>, Prob: iset<T> -> real) {
+    forall e1, e2 | e1 in eventSpace && e2 in eventSpace && e1 * e2 == iset{} :: Prob(e1) + Prob(e2) == Prob(e1 + e2)
+  }
+
+  // Definition 5
+  ghost predicate IsCountablyAdditive<T(!new)>(eventSpace: iset<iset<T>>, Prob: iset<T> -> real) {
+    forall f: nat -> iset<T> | (forall n :: f(n) in eventSpace) && (forall m, n | m != n :: f(m) * f(n) == iset{}) && (CountableUnion(f) in eventSpace) :: (CountableSum((n: nat) => Prob(f(n))) == Prob(CountableUnion(f)))
+  }
+
+  // Definition 6
+  ghost predicate IsMeasure<T(!new)>(eventSpace: iset<iset<T>>, sampleSpace: iset<T>, Prob: iset<T> -> real) {
+    && IsSigmaAlgebra(eventSpace, sampleSpace)
+    && IsPositive(eventSpace, Prob)
+    && IsCountablyAdditive(eventSpace, Prob)
+  }
+
+  ghost function PreImage<S(!new),T>(f: S -> T, e: iset<T>): iset<S> {
+    (iset s | f(s) in e)
+  }
+
+  // Definition 9
+  ghost predicate IsMeasurable<S(!new),T>(eventSpaceS: iset<iset<S>>, eventSpaceT: iset<iset<T>>, f: S -> T) {
+    forall e | e in eventSpaceT :: PreImage(f, e) in eventSpaceS
+  }
+
+  // Definition 10
+  ghost predicate IsMeasurePreserving<S(!new),T>(eventSpaceS: iset<iset<S>>, measureS: iset<S> -> real, eventSpaceT: iset<iset<T>>, measureT: iset<T> -> real, f: S -> T) {
+    && IsMeasurable(eventSpaceS, eventSpaceT, f)
+    && forall e | e in eventSpaceT :: measureS(PreImage(f, e)) == measureT(e)
+  }
+
+  // Definition 12
+  ghost predicate IsProbability<T(!new)>(eventSpace: iset<iset<T>>, sampleSpace: iset<T>, Prob: iset<T> -> real) {
+    && IsMeasure(eventSpace, sampleSpace, Prob)
+    && Prob(sampleSpace) == 1.0
+  }
+
+  // Definition 13
+  predicate AreIndepEvents<T>(eventSpace: iset<iset<T>>, Prob: iset<T> -> real, e1: iset<T>, e2: iset<T>) {
+    && (e1 in eventSpace)
+    && (e2 in eventSpace)
+    && (Prob(e1 * e2) == Prob(e1) * Prob(e2))
+  }
+
+  /*******
+   Lemmas
+  *******/
+
+  lemma boolsHaveSigmaAlgebra()
+    ensures IsSigmaAlgebra(boolEventSpace, boolSampleSpace)
+  {
+    forall e | e in boolEventSpace ensures e <= boolSampleSpace {
+      assert e <= boolSampleSpace by {
+        forall x: bool ensures x in e ==> x in boolSampleSpace {}
+      }
+    }
+  }
+
+  lemma natsHaveSigmaAlgebra()
+    ensures IsSigmaAlgebra(natEventSpace, natSampleSpace)
+  {}
+
+  lemma PreImageIdentity<S(!new)>(f: S -> S, e: iset<S>)
+    requires forall s: S :: f(s) == s
+    ensures PreImage(f, e) == e
+  {}
+
+  lemma PreImagesEqual<S(!new),T,U>(f: S -> T, e: iset<T>, f': S -> U, e': iset<U>)
+    requires forall s: S :: f(s) in e <==> f'(s) in e'
+    ensures PreImage(f, e) == PreImage(f', e')
+  {}
+
+  // Equation (2.18)
+  lemma PosCountAddImpliesAdd<T(!new)>(eventSpace: iset<iset<T>>, sampleSpace: iset<T>, Prob: iset<T> -> real)
+    requires IsSigmaAlgebra(eventSpace, sampleSpace)
+    requires IsPositive(eventSpace, Prob)
+    requires IsCountablyAdditive(eventSpace, Prob)
+    ensures IsAdditive(eventSpace, Prob)
+  {
+    forall e1, e2 | e1 in eventSpace && e2 in eventSpace && e1 * e2 == iset{} ensures Prob(e1) + Prob(e2) == Prob(e1 + e2) {
+      var f : nat -> iset<T> := (n: nat) => if n == 0 then e1 else if n == 1 then e2 else iset{};
+      assert CountableUnion(f) == e1 + e2;
+      assert CountableSum((n: nat) => Prob(f(n))) == Prob(e1) + Prob(e2) by {
+        assert CountableSum((n: nat) => Prob(f(n)), 2) == 0.0 by {
+          CountableSumOfZeroesIsZero((n: nat) => Prob(f(n)), 2);
+        }
+        calc {
+          CountableSum((n: nat) => Prob(f(n)))
+       ==
+          Prob(f(0)) + CountableSum((n: nat) => Prob(f(n)), 1)
+       ==
+          Prob(f(0)) + Prob(f(1)) + CountableSum((n: nat) => Prob(f(n)), 2)
+       ==
+          Prob(e1) + Prob(e2) + CountableSum((n: nat) => Prob(f(n)), 2)
+       ==
+          Prob(e1) + Prob(e2);
+        }
+      }
+      assert Prob(CountableUnion(f)) == CountableSum((n: nat) => Prob(f(n))) by {
+        assert IsCountablyAdditive(eventSpace, Prob);
+      }
+      assert Prob(e1 + e2) == Prob(e1) + Prob(e2);
+    }
+  }
+
+  lemma {:axiom} CountableSumOfZeroesIsZero(f: nat -> real, i: nat := 0)
+    requires forall n | n >= i :: f(n) == 0.0
+    ensures CountableSum(f, i) == 0.0
+
+  lemma CountableUnionSplit<T(!new)>(f: nat -> iset<T>, i: nat)
+    ensures CountableUnion(f, i) == f(i) + CountableUnion(f, i + 1)
+  {}
+
+  lemma BinaryUnion<T(!new)>(eventSpace: iset<iset<T>>, sampleSpace: iset<T>, e1: iset<T>, e2: iset<T>)
+    requires IsSigmaAlgebra(eventSpace, sampleSpace)
+    requires e1 in eventSpace
+    requires e2 in eventSpace
+    ensures e1 + e2 in eventSpace
+  {
+    var f : nat -> iset<T> := (n: nat) => if n == 0 then e1 else if n == 1 then e2 else iset{};
+    assert CountableUnion(f) == e1 + e2 by {
+      calc {
+        CountableUnion(f);
+      == { CountableUnionSplit(f, 0); }
+        e1 + CountableUnion(f, 1);
+      == { CountableUnionSplit(f, 1); }
+        e1 + e2;
+      }
+    }
+  }
+}
